Tactic_Inline.thy
@@ -11,6 +11,13 @@ lemma HIDDEN_EQ_ok:
   and   "HIDDEN_EQ v w \<Longrightarrow> HIDDEN_EQ (procargvars_add (Variable n) v) (procargvars_add (Variable n) w)"
 unfolding HIDDEN_EQ_def by simp_all *)
  
+lemma obs_eq'_rename_variables_proc:
+  assumes "obs_eq' V (callproc x (rename_local_variables_proc ren prc) args) body"
+  shows "obs_eq' V (callproc x prc args) body"
+using assms unfolding obs_eq'_def obs_eq_def rhoare_def denotation_callproc_rename_local_variables_proc .
+
+thm obs_eq'_rename_variables_proc[of _ _ "[]"]
+
 ML_file "tactic_inline.ML"
                                                                     
 method_setup inline = {*
